Extracting GPU.Ref

src/examples/GPU.Example1.fst
@@ -23,21 +23,21 @@ fn main (_:unit)
   ensures  cpu
 {
   let r  = Box.alloc #U64.t 1uL;
-  let gr = gpu_alloc0_u64 ();
+  let gr = gpu_alloc0 #U64.t ();
    
   Box.to_ref_pts_to r;
-  GPU.Ref.gpu_memcpy_host_to_device_u64  (Box.box_to_ref r) gr;
+  GPU.Ref.gpu_memcpy_host_to_device (Box.box_to_ref r) gr;
 
   launch_kernel_1 (fun () -> kernel gr #(hide 1uL));
 
-  GPU.Ref.gpu_memcpy_device_to_host_u64 (Box.box_to_ref r) gr;
+  GPU.Ref.gpu_memcpy_device_to_host (Box.box_to_ref r) gr;
   Box.to_box_pts_to r;
 
   let v = Pulse.Lib.Box.(!r);
    
   assert (pure (v == 2uL));
    
-  gpu_free_u64 gr;
+  gpu_free gr;
   Box.free r;
 }
 ```
