src/lib/GPU.Ref.fsti
@@ -3,6 +3,7 @@ module GPU.Ref
 open Pulse.Lib.Pervasives
 open FStar.Tactics.V2
 open GPU.Base
+open GPU.Types
 
 val gpu_ref (a:Type u#0) : Type u#0
 
@@ -13,86 +14,77 @@ val gpu_pts_to
   (v : a)
 : slprop
 
-val gpu_alloc0_u64
-  ()
-: stt (gpu_ref FStar.UInt64.t)
-      cpu
-      (fun x -> cpu ** (exists* (v:_). gpu_pts_to x v))
-
-val gpu_alloc0
+```pulse
+val fn gpu_alloc0
   (#a:Type u#0)
+  {| sized a |}
   ()
-: stt (gpu_ref a)
-      cpu
-      (fun x -> cpu ** (exists* (v:a). gpu_pts_to x v))
+  requires cpu
+  returns  x : gpu_ref a
+  ensures  cpu ** (exists* (v:a). gpu_pts_to x #1.0R v)
+```
 
-val gpu_alloc
-  (#a:Type u#0)
-  (v:a)
-: stt (gpu_ref a)
-      cpu
-      (fun x -> cpu ** gpu_pts_to x v)
+// ```pulse
+// val fn gpu_alloc
+//   (#a:Type u#0)
+//   {| sized a |}
+//   (v:a)
+//   requires cpu
+//   returns  x : gpu_ref a
+//   ensures  cpu ** gpu_pts_to x #1.0R v
+// ```
 
-val gpu_free
+```pulse
+val fn gpu_free
   (#a:Type u#0)
   (r : gpu_ref a)
   (#v : erased a)
-: stt unit
-      (cpu ** gpu_pts_to r v)
-      (fun _ -> cpu)
+  requires cpu ** gpu_pts_to r #1.0R v
+  ensures  cpu
+```
 
-val gpu_read (#a:Type u#0) (x:gpu_ref a) (#f:perm) (#v0:erased a)
-  : stt a (gpu ** gpu_pts_to x #f v0)
-          (fun v -> gpu ** gpu_pts_to x #f v ** pure (v == reveal v0))
-
-val gpu_write (#a:Type u#0) (x:gpu_ref a) (v:a)
-  : stt unit (gpu ** (exists* v0. gpu_pts_to x v0))
-             (fun _ -> gpu ** gpu_pts_to x v)
-
-(* cudaMemcpy (_, _, _, cudaMemcpyHostToDevice) *)
-val gpu_memcpy_host_to_device
+```pulse
+val fn gpu_read
   (#a:Type u#0)
+  (r : gpu_ref a)
+  (#f : perm)
+  (#v0 : erased a)
+  requires gpu ** gpu_pts_to r #f v0
+  returns  v : a
+  ensures  gpu ** gpu_pts_to r #f v ** pure (v == reveal v0)
+```
+
+```pulse
+val fn gpu_write
+  (#a:Type u#0)
+  (r : gpu_ref a)
+  (v : a)
+  requires gpu ** (exists* v0. gpu_pts_to r #1.0R v0)
+  ensures  gpu ** gpu_pts_to r #1.0R v
+```
+
+```pulse
+val fn gpu_memcpy_host_to_device
+  (#a:Type u#0)
+  {| sized a |}
   (r  : ref a)
+  (gr : gpu_ref a)
   (#f : perm)
   (#v : erased a)
-  (gr : gpu_ref a)
   (#gv : erased a)
-  : stt unit (cpu ** pts_to r #f v ** gpu_pts_to gr #1.0R gv)
-             (fun _ -> cpu ** pts_to r #f v ** gpu_pts_to gr #1.0R v)
+  requires cpu ** pts_to r #1.0R v ** gpu_pts_to gr #f gv
+  ensures  cpu ** pts_to r #1.0R v ** gpu_pts_to gr #f v
+```
 
-(* cudaMemcpy (_, _, _, cudaMemcpyDeviceToHost) *)
-val gpu_memcpy_device_to_host
+```pulse
+val fn gpu_memcpy_device_to_host
   (#a:Type u#0)
+  {| sized a |}
   (r  : ref a)
-  (#v : erased a)
   (gr : gpu_ref a)
-  (#f:perm)
-  (#gv : erased a)
-  : stt unit (cpu ** pts_to r #1.0R v ** gpu_pts_to gr #f gv)
-             (fun _ -> cpu ** pts_to r #1.0R gv ** gpu_pts_to gr #f gv)
-
-val gpu_memcpy_host_to_device_u64
-  (r  : ref FStar.UInt64.t)
   (#f : perm)
-  (#v : erased FStar.UInt64.t)
-  (gr : gpu_ref FStar.UInt64.t)
-  (#gv : erased FStar.UInt64.t)
-  : stt unit (cpu ** pts_to r #f v ** gpu_pts_to gr #1.0R gv)
-             (fun _ -> cpu ** pts_to r #f v ** gpu_pts_to gr #1.0R v)
-
-(* cudaMemcpy (_, _, _, cudaMemcpyDeviceToHost) *)
-val gpu_memcpy_device_to_host_u64
-  (r  : ref FStar.UInt64.t)
-  (#v : erased FStar.UInt64.t)
-  (gr : gpu_ref FStar.UInt64.t)
-  (#f:perm)
-  (#gv : erased FStar.UInt64.t)
-  : stt unit (cpu ** pts_to r #1.0R v ** gpu_pts_to gr #f gv)
-             (fun _ -> cpu ** pts_to r #1.0R gv ** gpu_pts_to gr #f gv)
-
-val gpu_free_u64
-  (r : gpu_ref FStar.UInt64.t)
-  (#v : erased FStar.UInt64.t)
-: stt unit
-      (cpu ** gpu_pts_to r v)
-      (fun _ -> cpu)
+  (#v : erased a)
+  (#gv : erased a)
+  requires cpu ** pts_to r #1.0R v ** gpu_pts_to gr #f gv
+  ensures  cpu ** pts_to r #1.0R gv ** gpu_pts_to gr #f gv
+```
